theories/Core/Semantic/PER.v
@@ -1,1 +1,0 @@
-From Mctt.Core.Semantic.PER Require Export CoreTactics Definitions Lemmas.
