theories/Core/Syntactic/WCong/Definitions.v
@@ -3,61 +3,61 @@ From Mctt.Core Require Import Base.
 From Mctt.Core.Syntactic.System Require Export Definitions.
 Import Syntax_Notations.
 
-Reserved Notation "⊢ M ≈≈ M'" 
+Reserved Notation "⊢ M ≈ M'" 
   (in custom judg at level 80, M custom exp, M' custom exp, no associativity). 
-Reserved Notation "⊢s σ ≈≈ σ'" 
+Reserved Notation "⊢s σ ≈ σ'" 
   (in custom judg at level 80, σ custom exp, σ' custom exp, no associativity). 
 
 Generalizable All Variables.
 
 Inductive exp_weak_cong : exp -> exp -> Prop :=
 | exp_wcong_type :
-  `( {{ ⊢ Type@i ≈≈ Type@i }} )
+  `( {{ ⊢ Type@i ≈ Type@i }} )
 | exp_wcong_nat :
-  {{ ⊢ ℕ ≈≈ ℕ }}
+  {{ ⊢ ℕ ≈ ℕ }}
 | exp_wcong_zero : 
-  {{ ⊢ zero ≈≈ zero }}
+  {{ ⊢ zero ≈ zero }}
 | exp_wcong_succ :
-  `( {{ ⊢ M ≈≈ M' }} ->
-     {{ ⊢ succ M ≈≈ succ M'}} )
+  `( {{ ⊢ M ≈ M' }} ->
+     {{ ⊢ succ M ≈ succ M'}} )
 | exp_wcong_rec : 
-  `( {{ ⊢ A ≈≈ A' }} ->
-     {{ ⊢ MZ ≈≈ MZ' }} ->
-     {{ ⊢ MS ≈≈ MS' }} ->
-     {{ ⊢ M ≈≈ M' }} ->
-     {{ ⊢ rec M return A | zero -> MZ | succ -> MS end ≈≈ rec M' return A' | zero -> MZ' | succ -> MS' end  }} )
+  `( {{ ⊢ A ≈ A' }} ->
+     {{ ⊢ MZ ≈ MZ' }} ->
+     {{ ⊢ MS ≈ MS' }} ->
+     {{ ⊢ M ≈ M' }} ->
+     {{ ⊢ rec M return A | zero -> MZ | succ -> MS end ≈ rec M' return A' | zero -> MZ' | succ -> MS' end  }} )
 | exp_wcong_pi : 
-  `( {{ ⊢ A ≈≈ A' }} ->
-     {{ ⊢ B ≈≈ B' }} ->
-     {{ ⊢ Π A B ≈≈ Π A' B' }} )
+  `( {{ ⊢ A ≈ A' }} ->
+     {{ ⊢ B ≈ B' }} ->
+     {{ ⊢ Π A B ≈ Π A' B' }} )
 | exp_wcong_fn : 
-  `( {{ ⊢ M ≈≈ M' }} ->
-     {{ ⊢ λ A M ≈≈ λ A' M' }} )
+  `( {{ ⊢ M ≈ M' }} ->
+     {{ ⊢ λ A M ≈ λ A' M' }} )
 | exp_wcong_app : 
-  `( {{ ⊢ M ≈≈ M' }} ->
-     {{ ⊢ N ≈≈ N' }} ->
-     {{ ⊢ M N ≈≈ M' N' }} )
+  `( {{ ⊢ M ≈ M' }} ->
+     {{ ⊢ N ≈ N' }} ->
+     {{ ⊢ M N ≈ M' N' }} )
 | exp_wcong_var : 
-  `( {{ ⊢ #x ≈≈ #x }} )
+  `( {{ ⊢ #x ≈ #x }} )
 | exp_wcong_sub : 
-  `( {{ ⊢ M ≈≈ M' }} ->
-     {{ ⊢s σ ≈≈ σ' }} ->
-     {{ ⊢ M[σ] ≈≈ M'[σ'] }} )
-where "⊢ M ≈≈ M'" := (exp_weak_cong M M') (in custom judg) : type_scope
+  `( {{ ⊢ M ≈ M' }} ->
+     {{ ⊢s σ ≈ σ' }} ->
+     {{ ⊢ M[σ] ≈ M'[σ'] }} )
+where "⊢ M ≈ M'" := (exp_weak_cong M M') (in custom judg) : type_scope
 with subst_weak_cong : sub -> sub -> Prop :=
 | subst_wcong_id : 
-  {{ ⊢s Id ≈≈ Id }}
+  {{ ⊢s Id ≈ Id }}
 | subst_wcong_weaken :
-  `( {{ ⊢s Wk ≈≈ Wk }} )
+  `( {{ ⊢s Wk ≈ Wk }} )
 | subst_wcong_compose :
-  `( {{ ⊢s τ ≈≈ τ' }} ->
-     {{ ⊢s σ ≈≈ σ' }} ->
-     {{ ⊢s σ ∘ τ ≈≈ σ' ∘ τ' }} )
+  `( {{ ⊢s τ ≈ τ' }} ->
+     {{ ⊢s σ ≈ σ' }} ->
+     {{ ⊢s σ ∘ τ ≈ σ' ∘ τ' }} )
 | subst_wcong_extend :
-  `( {{ ⊢s σ ≈≈ σ' }} ->
-     {{ ⊢ M ≈≈ M' }} ->
-     {{ ⊢s (σ ,, M) ≈≈ (σ' ,, M') }} )
-where "⊢s σ ≈≈ σ'" := (subst_weak_cong σ σ') (in custom judg) : type_scope.
+  `( {{ ⊢s σ ≈ σ' }} ->
+     {{ ⊢ M ≈ M' }} ->
+     {{ ⊢s (σ ,, M) ≈ (σ' ,, M') }} )
+where "⊢s σ ≈ σ'" := (subst_weak_cong σ σ') (in custom judg) : type_scope.
 
 #[export]
 Hint Constructors exp_weak_cong subst_weak_cong : mctt.
@@ -68,46 +68,46 @@ Combined Scheme syntactic_wcong_mut_ind from
   exp_weak_cong_mut_ind,
   subst_weak_cong_mut_ind.
 
-Reserved Notation "⊢nf M ≈≈ M'" 
+Reserved Notation "⊢nf M ≈ M'" 
   (in custom judg at level 80, M custom nf, M' custom nf, no associativity). 
-Reserved Notation "⊢ne N ≈≈ N'" 
+Reserved Notation "⊢ne N ≈ N'" 
   (in custom judg at level 80, N custom nf, N' custom nf, no associativity). 
 
 Inductive nf_weak_cong : nf -> nf -> Prop :=
 | nf_wcong_type :
-  `({{ ⊢nf Type@i ≈≈ Type@i }} )
+  `({{ ⊢nf Type@i ≈ Type@i }} )
 | nf_wcong_nat :
-  {{ ⊢nf ℕ ≈≈ ℕ }}
+  {{ ⊢nf ℕ ≈ ℕ }}
 | nf_wcong_zero : 
-  {{ ⊢nf zero ≈≈ zero }}
+  {{ ⊢nf zero ≈ zero }}
 | nf_wcong_succ :
-  `( {{ ⊢nf M ≈≈ M' }} ->
-     {{ ⊢nf succ M ≈≈ succ M'}} )
+  `( {{ ⊢nf M ≈ M' }} ->
+     {{ ⊢nf succ M ≈ succ M'}} )
 | nf_wcong_pi : 
-  `( {{ ⊢nf A ≈≈ A' }} ->
-     {{ ⊢nf B ≈≈ B' }} ->
-     {{ ⊢nf Π A B ≈≈ Π A' B' }} )
+  `( {{ ⊢nf A ≈ A' }} ->
+     {{ ⊢nf B ≈ B' }} ->
+     {{ ⊢nf Π A B ≈ Π A' B' }} )
 | nf_wcong_fn : 
-  `( {{ ⊢nf M ≈≈ M' }} ->
-     {{ ⊢nf λ A M ≈≈ λ A' M' }} )
+  `( {{ ⊢nf M ≈ M' }} ->
+     {{ ⊢nf λ A M ≈ λ A' M' }} )
 | nf_wcong_neut : 
-  `( {{ ⊢ne M ≈≈ M' }} ->
-     {{ ⊢nf ⇑ M ≈≈ ⇑ M' }} )
-where "⊢nf M ≈≈ M'" := (nf_weak_cong M M') (in custom judg) : type_scope
+  `( {{ ⊢ne M ≈ M' }} ->
+     {{ ⊢nf ⇑ M ≈ ⇑ M' }} )
+where "⊢nf M ≈ M'" := (nf_weak_cong M M') (in custom judg) : type_scope
 with ne_weak_cong : ne -> ne -> Prop :=
 | ne_wcong_netrec : 
-  `( {{ ⊢nf A ≈≈ A' }} ->
-     {{ ⊢nf MZ ≈≈ MZ' }} ->
-     {{ ⊢nf MS ≈≈ MS' }} ->
-     {{ ⊢ne M ≈≈ M' }} ->
-     {{ ⊢ne rec M return A | zero -> MZ | succ -> MS end ≈≈ rec M' return A' | zero -> MZ' | succ -> MS' end  }} )
+  `( {{ ⊢nf A ≈ A' }} ->
+     {{ ⊢nf MZ ≈ MZ' }} ->
+     {{ ⊢nf MS ≈ MS' }} ->
+     {{ ⊢ne M ≈ M' }} ->
+     {{ ⊢ne rec M return A | zero -> MZ | succ -> MS end ≈ rec M' return A' | zero -> MZ' | succ -> MS' end  }} )
 | ne_wcong_app :
-  `( {{ ⊢ne M ≈≈ M' }} ->
-     {{ ⊢nf N ≈≈ N' }} ->
-     {{ ⊢ne M N ≈≈ M' N' }} )
+  `( {{ ⊢ne M ≈ M' }} ->
+     {{ ⊢nf N ≈ N' }} ->
+     {{ ⊢ne M N ≈ M' N' }} )
 | ne_wcong_var : 
-  `( {{ ⊢ne #x ≈≈ #x }} )
-where "⊢ne N ≈≈ N'" := (ne_weak_cong N N') (in custom judg) : type_scope.
+  `( {{ ⊢ne #x ≈ #x }} )
+where "⊢ne N ≈ N'" := (ne_weak_cong N N') (in custom judg) : type_scope.
 
 #[export]
 Hint Constructors nf_weak_cong ne_weak_cong : mctt.
